restore output buffer, with cleaner state-machine-like interface

steel/Zeta.Steel.ExternalPtr.fsti
@@ -9,17 +9,79 @@ module U8 = FStar.UInt8
 open Steel.ST.Util
 
 inline_for_extraction
-val extern_input_ptr : Type0
+val extern_ptr : Type0
 
-val has_extern_input_ptr (e: extern_input_ptr) (n: U32.t) : vprop
+[@@erasable]
+noeq
+type state =
+| Unknown: (in_contents: Seq.seq U8.t) -> state
+| Unread: (in_contents: Seq.seq U8.t) -> (out_len: U32.t) -> state
+| Read: (in_contents: Seq.seq U8.t) -> (out_len: U32.t) -> state
+| Written: (written: Seq.seq U8.t) -> state
+
+let get_in_contents
+  (s: state)
+: Ghost (Seq.seq U8.t)
+    (requires (~ (Written? s)))
+    (ensures (fun _ -> True))
+= match s with
+  | Unknown in_contents
+  | Unread in_contents _
+  | Read in_contents _
+    -> in_contents
+
+val extern_in_out_pts_to (e1: extern_ptr) (e2: extern_ptr) (s: state) : vprop
+
+let is_valid_state (b: bool) (in_contents: Seq.seq U8.t) (out_len: U32.t) : Tot state =
+  if b then Unread in_contents out_len else Unknown in_contents
+
+val extern_in_out_pts_to_is_valid
+  (e1: extern_ptr)
+  (w1: Ghost.erased (Seq.seq U8.t))
+  (n1: U32.t)
+  (e2: extern_ptr)
+  (n2: U32.t)
+: ST bool
+  (extern_in_out_pts_to e1 e2 (Unknown w1))
+  (fun b -> extern_in_out_pts_to e1 e2 (is_valid_state b w1 n2))
+  True
+  (fun b -> b == true ==> (
+    U32.v n1 == Seq.length w1
+  ))
 
 inline_for_extraction
 val copy_extern_input_ptr
-  (e: extern_input_ptr)
+  (e1: extern_ptr)
+  (w1: Ghost.erased (Seq.seq U8.t))
+  (e2: extern_ptr)
+  (n: U32.t)
+  (out_len: Ghost.erased U32.t)
+  (a: A.array U8.t)
+: ST unit
+    (extern_in_out_pts_to e1 e2 (Unread w1 out_len) `star` exists_ (fun contents -> A.pts_to a full_perm contents))
+    (fun _ ->
+      extern_in_out_pts_to e1 e2 (Read w1 out_len) `star` A.pts_to a full_perm w1
+    )
+    (A.length a == U32.v n \/
+      Seq.length w1 == U32.v n
+    )
+    (fun _ -> True)
+
+inline_for_extraction
+val copy_extern_output_ptr
+  (e1: extern_ptr)
+  (w1: Ghost.erased (Seq.seq U8.t))
+  (e2: extern_ptr)
   (n: U32.t)
   (a: A.array U8.t)
-: ST bool
-    (has_extern_input_ptr e n `star` exists_ (fun contents -> A.pts_to a full_perm contents))
-    (fun _ -> has_extern_input_ptr e n `star` exists_ (fun contents -> A.pts_to a full_perm contents))
-    (A.length a == U32.v n)
+  (p: perm)
+  (contents: Ghost.erased (Seq.seq U8.t))
+: ST unit
+    (extern_in_out_pts_to e1 e2 (Read w1 n) `star` A.pts_to a p contents)
+    (fun _ ->
+      extern_in_out_pts_to e1 e2 (Written contents) `star` A.pts_to a p contents
+    )
+    (A.length a == U32.v n \/
+      Seq.length contents == U32.v n
+    )
     (fun _ -> True)
